more

Weidenbach_Book/Watched_Literals_Initialisation.thy
@@ -43,7 +43,7 @@ fun add_empty_conflict_init :: \<open>'v twl_st_init \<Rightarrow> 'v twl_st_ini
        ((M, N, U, Some {#}, NE, UE, WS, {#}), add_mset {#} OC)\<close>
 
 fun add_to_clauses_init :: \<open>'v clause_l \<Rightarrow> 'v twl_st_init \<Rightarrow> 'v twl_st_init\<close> where
-   \<open>add_to_clauses_init C ((M, N, U, D, NE, UE, WS, Q), OC) = 
+   \<open>add_to_clauses_init C ((M, N, U, D, NE, UE, WS, Q), OC) =
         ((M, add_mset (twl_clause_of C) N, U, D, NE, UE, WS, Q), OC)\<close>
 
 type_synonym 'v twl_st_l_init = \<open>'v twl_st_l \<times> 'v clauses\<close>
@@ -53,6 +53,12 @@ fun get_trail_l_init :: \<open>'v twl_st_l_init \<Rightarrow> ('v, nat) ann_lit 
 
 fun get_conflict_l_init :: \<open>'v twl_st_l_init \<Rightarrow> 'v cconflict\<close> where
   \<open>get_conflict_l_init ((_, _, D, _, _, _, _), _) = D\<close>
+
+fun get_unit_clauses_l_init :: \<open>'v twl_st_l_init \<Rightarrow> 'v clauses\<close> where
+  \<open>get_unit_clauses_l_init ((M, N, D, NE, UE, WS, Q), _) = NE + UE\<close>
+
+fun get_learned_unit_clauses_l_init :: \<open>'v twl_st_l_init \<Rightarrow> 'v clauses\<close> where
+  \<open>get_learned_unit_clauses_l_init ((M, N, D, NE, UE, WS, Q), _) = UE\<close>
 
 fun get_clauses_l_init :: \<open>'v twl_st_l_init \<Rightarrow> 'v clauses_l\<close> where
   \<open>get_clauses_l_init ((M, N, D, NE, UE, WS, Q), _) = N\<close>
@@ -247,24 +253,28 @@ lemma init_dt_pre_ConsD: \<open>init_dt_pre (a # CS) SOC \<Longrightarrow> init_
   by fastforce
 
 definition init_dt_spec where
-  \<open>init_dt_spec CS SOC = (\<lambda>(S', OC'). 
-       \<exists>T'. ((S', OC'), T') \<in> twl_st_l_init \<and>
+  \<open>init_dt_spec CS SOC SOC' \<longleftrightarrow>
+     (\<exists>T'. (SOC', T') \<in> twl_st_l_init \<and>
            twl_struct_invs_init T' \<and>
-           clauses_to_update_l S' = {#} \<and>
-           (\<forall>s\<in>set (get_trail_l S'). \<not>is_decided s) \<and>
-           (get_conflict_l S' = None \<longrightarrow>
-              literals_to_update_l S' = uminus `# lit_of `# mset (get_trail_l S')) \<and>
-           (mset `# mset CS + mset `# ran_mf (get_clauses_l (fst SOC)) + snd SOC =
-              mset `# ran_mf (get_clauses_l S') + OC') \<and>
-           learned_clss_lf (get_clauses_l (fst SOC)) = learned_clss_lf (get_clauses_l S') \<and>
-           twl_list_invs S' \<and>
+           clauses_to_update_l_init SOC' = {#} \<and>
+           (\<forall>s\<in>set (get_trail_l_init SOC'). \<not>is_decided s) \<and>
+           (get_conflict_l_init SOC' = None \<longrightarrow>
+              literals_to_update_l_init SOC' = uminus `# lit_of `# mset (get_trail_l_init SOC')) \<and>
+           (mset `# mset CS + mset `# ran_mf (get_clauses_l_init SOC) + other_clauses_l_init SOC +
+                 get_unit_clauses_l_init SOC =
+            mset `# ran_mf (get_clauses_l_init SOC') + other_clauses_l_init SOC'  +
+                 get_unit_clauses_l_init SOC') \<and>
+           learned_clss_lf (get_clauses_l_init SOC) = learned_clss_lf (get_clauses_l_init SOC') \<and>
+           get_learned_unit_clauses_l_init SOC' = get_learned_unit_clauses_l_init SOC \<and>
+           twl_list_invs (fst SOC') \<and>
            twl_stgy_invs (fst T') \<and>
-           (OC' \<noteq> {#} \<longrightarrow> get_conflict_l S' \<noteq> None) \<and>
-           ({#} \<in># mset `# mset CS \<longrightarrow> get_conflict_l S' \<noteq> None))\<close>
+           (other_clauses_l_init SOC' \<noteq> {#} \<longrightarrow> get_conflict_l_init SOC' \<noteq> None) \<and>
+           ({#} \<in># mset `# mset CS \<longrightarrow> get_conflict_l_init SOC' \<noteq> None) \<and>
+           (get_conflict_l_init SOC \<noteq> None \<longrightarrow> get_conflict_l_init SOC = get_conflict_l_init SOC'))\<close>
 
 
 lemma twl_struct_invs_init_add_to_other_init:
-  assumes 
+  assumes
     dist: \<open>distinct a\<close> and
     lev: \<open>count_decided (get_trail (fst T)) = 0\<close> and
     invs: \<open>twl_struct_invs_init T\<close>
@@ -277,7 +287,7 @@ proof -
     by (cases T) auto
   have \<open>cdcl\<^sub>W_restart_mset.cdcl\<^sub>W_all_struct_inv (M, clauses N + NE + OC, clauses U + UE, D)\<close>
     using invs unfolding T twl_struct_invs_init_def by auto
-  then have [simp]: 
+  then have [simp]:
    \<open>cdcl\<^sub>W_restart_mset.cdcl\<^sub>W_all_struct_inv (M, add_mset (mset a) (clauses N + NE + OC), clauses U + UE, D)\<close>
     using dist
     by (auto simp: cdcl\<^sub>W_restart_mset.cdcl\<^sub>W_all_struct_inv_def
@@ -312,7 +322,7 @@ lemma invariants_init_state:
   shows \<open>propa_cands_enqueued (fst T)\<close> and \<open>confl_cands_enqueued (fst T)\<close> and \<open>twl_st_inv (fst T)\<close>
     \<open>clauses_to_update_inv (fst T)\<close> and \<open>past_invs (fst T)\<close> and \<open>distinct_queued (fst T)\<close> and
     \<open>valid_enqueued (fst T)\<close> and \<open>twl_st_exception_inv (fst T)\<close> and \<open>no_duplicate_queued (fst T)\<close>
-proof -    
+proof -
   obtain M N U NE UE OC D where
     T: \<open>T = ((M, N, U, D, NE, UE, {#}, uminus `# lit_of `# mset M), OC)\<close>
     using MQ WS by (cases T) auto
@@ -386,7 +396,7 @@ proof -
     apply - apply (intro conjI impI allI)
     apply (case_tac x; cases D)
     by (auto simp: T twl_exception_inv.simps lits_of_def uminus_lit_swap)
-  
+
   show \<open>no_duplicate_queued (fst T)\<close>
     by (auto simp: T)
 qed
@@ -405,7 +415,7 @@ lemma twl_struct_invs_init_init_state:
 proof -
   have n_d: \<open>no_dup (get_trail_init T)\<close>
     using struct_invs unfolding  cdcl\<^sub>W_restart_mset.cdcl\<^sub>W_all_struct_inv_def
-      cdcl\<^sub>W_restart_mset.cdcl\<^sub>W_M_level_inv_def by (cases T) (auto simp: trail.simps) 
+      cdcl\<^sub>W_restart_mset.cdcl\<^sub>W_M_level_inv_def by (cases T) (auto simp: trail.simps)
   then show ?thesis
     using invariants_init_state[OF lev wf MQ WS n_d] assms unfolding twl_struct_invs_init_def
     by fast+
@@ -413,7 +423,7 @@ qed
 
 
 lemma twl_struct_invs_init_add_to_unit_init_clauses:
-  assumes 
+  assumes
     dist: \<open>distinct a\<close> and
     lev: \<open>count_decided (get_trail (fst T)) = 0\<close> and
     invs: \<open>twl_struct_invs_init T\<close> and
@@ -427,7 +437,7 @@ proof -
     by (cases T) auto
   have \<open>cdcl\<^sub>W_restart_mset.cdcl\<^sub>W_all_struct_inv (M, clauses N + NE + OC, clauses U + UE, D)\<close>
     using invs unfolding T twl_struct_invs_init_def by auto
-  then have [simp]: 
+  then have [simp]:
    \<open>cdcl\<^sub>W_restart_mset.cdcl\<^sub>W_all_struct_inv (M, add_mset (mset a) (clauses N + NE + OC), clauses U + UE, D)\<close>
     using twl_struct_invs_init_add_to_other_init[OF dist lev invs]
     unfolding T twl_struct_invs_init_def
@@ -465,7 +475,7 @@ proof -
 qed
 
 lemma twl_struct_invs_init_set_conflict_init:
-  assumes 
+  assumes
     dist: \<open>distinct C\<close> and
     lev: \<open>count_decided (get_trail (fst T)) = 0\<close> and
     invs: \<open>twl_struct_invs_init T\<close> and
@@ -480,7 +490,7 @@ proof -
     by (cases T) auto
   have \<open>cdcl\<^sub>W_restart_mset.cdcl\<^sub>W_all_struct_inv (M, clauses N + NE + OC, clauses U + UE, D)\<close>
     using invs unfolding T twl_struct_invs_init_def by auto
-  then have [simp]: 
+  then have [simp]:
    \<open>cdcl\<^sub>W_restart_mset.cdcl\<^sub>W_all_struct_inv (M, add_mset (mset C) (clauses N + NE + OC),
         clauses U + UE, Some (mset C))\<close>
     using dist ex
@@ -547,7 +557,7 @@ proof -
     excep: \<open>twl_st_exception_inv (M, N, U, None, NE, UE, WS, ?Q)\<close> and
     st_inv: \<open>twl_st_inv (M, N, U, None, NE, UE, WS, ?Q)\<close>
     using invs confl unfolding T twl_struct_invs_init_def by auto
-  then have [simp]: 
+  then have [simp]:
    \<open>cdcl\<^sub>W_restart_mset.cdcl\<^sub>W_all_struct_inv (M, add_mset {#L#} (clauses N + NE + OC),
      clauses U + UE, None)\<close> and
    n_d: \<open>no_dup M\<close>
@@ -556,7 +566,7 @@ proof -
        cdcl\<^sub>W_restart_mset.cdcl\<^sub>W_M_level_inv_def cdcl\<^sub>W_restart_mset.cdcl\<^sub>W_conflicting_def
        cdcl\<^sub>W_restart_mset.distinct_cdcl\<^sub>W_state_def all_decomposition_implies_def
        clauses_def cdcl\<^sub>W_restart_mset.cdcl\<^sub>W_learned_clause_def)
-  then have [simp]: 
+  then have [simp]:
    \<open>cdcl\<^sub>W_restart_mset.cdcl\<^sub>W_all_struct_inv (Propagated L {#L#} # M,
         add_mset {#L#} (clauses N + NE + OC), clauses U + UE, None)\<close>
     using undef by (auto simp: cdcl\<^sub>W_restart_mset.cdcl\<^sub>W_all_struct_inv_def T H
@@ -614,6 +624,10 @@ lemma [twl_st_l_init]:
   \<open>other_clauses_l_init (already_propagated_unit_init_l C S) = other_clauses_l_init S\<close>
   \<open>clauses_to_update_l_init (already_propagated_unit_init_l C S) = clauses_to_update_l_init S\<close>
   \<open>literals_to_update_l_init (already_propagated_unit_init_l C S) = literals_to_update_l_init S\<close>
+  \<open>get_clauses_l_init (already_propagated_unit_init_l C S) = get_clauses_l_init S\<close>
+  \<open>get_unit_clauses_l_init (already_propagated_unit_init_l C S) = add_mset C (get_unit_clauses_l_init S)\<close>
+  \<open>get_learned_unit_clauses_l_init (already_propagated_unit_init_l C S) =
+       get_learned_unit_clauses_l_init S\<close>
   \<open>get_conflict_l_init (T, OC) = get_conflict_l T\<close>
   by (solves \<open>cases S; cases T; auto simp: already_propagated_unit_init_l_def\<close>)+
 
@@ -644,13 +658,15 @@ lemma entailed_clss_inv_add_to_unit_init_clauses:
   by (cases T; cases C; auto simp: twl_st_inv.simps twl_exception_inv.simps)
 
 lemma init_dt_pre_already_propagated_unit_init_l:
-  assumes 
+  assumes
     hd_C: \<open>hd C \<in> lits_of_l (get_trail_l_init S)\<close> and
     pre: \<open>init_dt_pre CS S\<close> and
     nempty: \<open>C \<noteq> []\<close> and
     dist_C: \<open>distinct C\<close> and
     lev: \<open>count_decided (get_trail_l_init S) = 0\<close>
-  shows \<open>init_dt_pre CS (already_propagated_unit_init_l (mset C) S)\<close>
+  shows
+    \<open>init_dt_pre CS (already_propagated_unit_init_l (mset C) S)\<close> (is ?pre) and
+    \<open>init_dt_spec [C] S (already_propagated_unit_init_l (mset C) S)\<close>  (is ?spec)
 proof -
   obtain T where
     SOC_T: \<open>(S, T) \<in> twl_st_l_init\<close> and
@@ -688,10 +704,15 @@ proof -
     apply (rule twl_struct_invs_init_add_to_unit_init_clauses)
     using inv hd_C nempty dist_C lev SOC_T dec
     by (auto simp: twl_st_init count_decided_0_iff)
-  show ?thesis
+  show ?pre
     unfolding init_dt_pre_def
     apply (rule exI[of _ \<open>add_to_unit_init_clauses (mset C) T\<close>])
     using dist WS dec in_literals_to_update OC'_empty by (auto simp: twl_st_init twl_st_l_init)
+  show ?spec
+    unfolding init_dt_spec_def
+    apply (rule exI[of _ \<open>add_to_unit_init_clauses (mset C) T\<close>])
+    using dist WS dec in_literals_to_update OC'_empty nempty
+    by (auto simp: twl_st_init twl_st_l_init)
 qed
 
 lemma (in -) uminus_list_of_mset_convert_lits_l:
@@ -709,19 +730,25 @@ lemma (in -) twl_stgy_invs_backtrack_lvl_0:
 lemma [twl_st_l_init]:
   \<open>clauses_to_update_l_init (propagate_unit_init_l L S) =  clauses_to_update_l_init S\<close>
   \<open>get_trail_l_init (propagate_unit_init_l L S) = Propagated L 0 # get_trail_l_init S\<close>
-  \<open>literals_to_update_l_init (propagate_unit_init_l L S) = add_mset (-L) (literals_to_update_l_init S)\<close>
+  \<open>literals_to_update_l_init (propagate_unit_init_l L S) =
+     add_mset (-L) (literals_to_update_l_init S)\<close>
   \<open>get_conflict_l_init (propagate_unit_init_l L S) = get_conflict_l_init S\<close>
   \<open>clauses_to_update_l_init (propagate_unit_init_l L S) = clauses_to_update_l_init S\<close>
   \<open>other_clauses_l_init (propagate_unit_init_l L S) = other_clauses_l_init S\<close>
+  \<open>get_clauses_l_init (propagate_unit_init_l L S) = get_clauses_l_init S\<close>
+  \<open>get_learned_unit_clauses_l_init (propagate_unit_init_l L S) = get_learned_unit_clauses_l_init S\<close>
+  \<open>get_unit_clauses_l_init (propagate_unit_init_l L S) = add_mset {#L#} (get_unit_clauses_l_init S)\<close>
   by (cases S; auto simp: propagate_unit_init_l_def; fail)+
 
 lemma init_dt_pre_propagate_unit_init:
-  assumes 
+  assumes
     hd_C: \<open>undefined_lit (get_trail_l_init S) L\<close> and
     pre: \<open>init_dt_pre CS S\<close> and
     lev: \<open>count_decided (get_trail_l_init S) = 0\<close> and
     confl: \<open>get_conflict_l_init S = None\<close>
-  shows \<open>init_dt_pre CS (propagate_unit_init_l L S)\<close>
+  shows
+    \<open>init_dt_pre CS (propagate_unit_init_l L S)\<close> (is ?pre) and
+    \<open>init_dt_spec [[L]] S (propagate_unit_init_l L S)\<close> (is ?spec)
 proof -
   obtain T where
     SOC_T: \<open>(S, T) \<in> twl_st_l_init\<close> and
@@ -759,8 +786,13 @@ proof -
   have [simp]: \<open>twl_list_invs (fst (propagate_unit_init_l L S))\<close>
     using add_inv
     by (auto simp: S twl_list_invs_def propagate_unit_init_l_def)
-  show ?thesis
+  show ?pre
     unfolding init_dt_pre_def
+    apply (rule exI[of _ \<open>propagate_unit_init L T\<close>])
+    using dist WS dec in_literals_to_update OC'_empty confl
+    by (auto simp: twl_st_init twl_st_l_init)
+  show ?spec
+    unfolding init_dt_spec_def
     apply (rule exI[of _ \<open>propagate_unit_init L T\<close>])
     using dist WS dec in_literals_to_update OC'_empty confl
     by (auto simp: twl_st_init twl_st_l_init)
@@ -771,15 +803,21 @@ lemma [twl_st_l_init]:
   \<open>literals_to_update_l_init (set_conflict_init_l C S) = {#}\<close>
   \<open>clauses_to_update_l_init (set_conflict_init_l C S) = {#}\<close>
   \<open>get_conflict_l_init (set_conflict_init_l C S) = Some (mset C)\<close>
-  by (cases S; auto simp: set_conflict_init_l_def)+
+  \<open>get_unit_clauses_l_init (set_conflict_init_l C S) = add_mset (mset C) (get_unit_clauses_l_init S)\<close>
+  \<open>get_learned_unit_clauses_l_init (set_conflict_init_l C S) = get_learned_unit_clauses_l_init S\<close>
+  \<open>get_clauses_l_init (set_conflict_init_l C S) = get_clauses_l_init S\<close>
+  \<open>other_clauses_l_init (set_conflict_init_l C S) = other_clauses_l_init S\<close>
+  by (cases S; auto simp: set_conflict_init_l_def; fail)+
 
 lemma init_dt_pre_set_conflict_init_l:
-  assumes 
-    \<open>get_conflict_l_init S = None\<close> and
+  assumes
+    [simp]: \<open>get_conflict_l_init S = None\<close> and
     pre: \<open>init_dt_pre (C # CS) S\<close> and
     false: \<open>\<forall>L \<in> set C.  -L \<in> lits_of_l (get_trail_l_init S)\<close> and
     nempty: \<open>C \<noteq> []\<close>
-  shows \<open>init_dt_pre CS (set_conflict_init_l C S)\<close>
+  shows
+    \<open>init_dt_pre CS (set_conflict_init_l C S)\<close> (is ?pre) and
+    \<open>init_dt_spec [C] S (set_conflict_init_l C S)\<close> (is ?spec)
 proof -
   obtain T where
     SOC_T: \<open>(S, T) \<in> twl_st_l_init\<close> and
@@ -820,8 +858,12 @@ proof -
     apply (rule twl_struct_invs_init_set_conflict_init)
     using inv nempty dist_C SOC_T dec false nempty
     by (auto simp: twl_st_init count_decided_0_iff)
-  show ?thesis
+  show ?pre
     unfolding init_dt_pre_def
+    apply (rule exI[of _ \<open>set_conflict_init C T\<close>])
+    using dist WS dec in_literals_to_update OC'_empty by (auto simp: twl_st_init twl_st_l_init)
+  show ?spec
+    unfolding init_dt_spec_def
     apply (rule exI[of _ \<open>set_conflict_init C T\<close>])
     using dist WS dec in_literals_to_update OC'_empty by (auto simp: twl_st_init twl_st_l_init)
 qed
@@ -838,10 +880,14 @@ lemma [twl_st_l_init]:
   \<open>get_conflict_l_init (add_empty_conflict_init_l  T) = Some {#}\<close>
   \<open>clauses_to_update_l_init (add_empty_conflict_init_l T) =  clauses_to_update_l_init T\<close>
   \<open>literals_to_update_l_init (add_empty_conflict_init_l T) = {#}\<close>
+  \<open>get_unit_clauses_l_init (add_empty_conflict_init_l T) = get_unit_clauses_l_init T\<close>
+  \<open>get_learned_unit_clauses_l_init (add_empty_conflict_init_l T) = get_learned_unit_clauses_l_init T\<close>
+  \<open>get_clauses_l_init (add_empty_conflict_init_l T) = get_clauses_l_init T\<close>
+  \<open>other_clauses_l_init (add_empty_conflict_init_l T) = add_mset {#} (other_clauses_l_init T)\<close>
   by (cases T; auto simp: add_empty_conflict_init_l_def; fail)+
 
 lemma twl_struct_invs_init_add_empty_conflict_init_l:
-  assumes 
+  assumes
     lev: \<open>count_decided (get_trail (fst T)) = 0\<close> and
     invs: \<open>twl_struct_invs_init T\<close> and
     WS: \<open>clauses_to_update_init T = {#}\<close>
@@ -853,7 +899,7 @@ proof -
     using WS by (cases T) auto
   have \<open>cdcl\<^sub>W_restart_mset.cdcl\<^sub>W_all_struct_inv (M, clauses N + NE + OC, clauses U + UE, D)\<close>
     using invs unfolding T twl_struct_invs_init_def by auto
-  then have [simp]: 
+  then have [simp]:
    \<open>cdcl\<^sub>W_restart_mset.cdcl\<^sub>W_all_struct_inv (M, add_mset {#} (clauses N + NE + OC),
         clauses U + UE, Some {#})\<close>
     unfolding T twl_struct_invs_init_def
@@ -891,10 +937,12 @@ proof -
 qed
 
 lemma init_dt_pre_add_empty_conflict_init_l:
-  assumes 
-    \<open>get_conflict_l_init S = None\<close> and
+  assumes
+    confl[simp]: \<open>get_conflict_l_init S = None\<close> and
     pre: \<open>init_dt_pre ([] # CS) S\<close>
-  shows \<open>init_dt_pre CS (add_empty_conflict_init_l S)\<close>
+  shows
+    \<open>init_dt_pre CS (add_empty_conflict_init_l S)\<close> (is ?pre)
+    \<open>init_dt_spec [[]] S (add_empty_conflict_init_l S)\<close> (is ?spec)
 proof -
   obtain T where
     SOC_T: \<open>(S, T) \<in> twl_st_l_init\<close> and
@@ -934,8 +982,12 @@ proof -
     apply (rule twl_struct_invs_init_add_empty_conflict_init_l)
     using inv SOC_T dec WS
     by (auto simp: twl_st_init twl_st_l_init count_decided_0_iff uminus_list_of_mset_convert_lits_l)
-  show ?thesis
+  show ?pre
     unfolding init_dt_pre_def
+    apply (rule exI[of _ \<open>add_empty_conflict_init T\<close>])
+    using dist WS dec in_literals_to_update OC'_empty by (auto simp: twl_st_init twl_st_l_init)
+  show ?spec
+    unfolding init_dt_spec_def
     apply (rule exI[of _ \<open>add_empty_conflict_init T\<close>])
     using dist WS dec in_literals_to_update OC'_empty by (auto simp: twl_st_init twl_st_l_init)
 qed
@@ -984,7 +1036,7 @@ proof -
     excep: \<open>twl_st_exception_inv (M, N, U, None, NE, UE, WS, ?Q)\<close> and
     st_inv: \<open>twl_st_inv (M, N, U, None, NE, UE, WS, ?Q)\<close>
     using invs confl unfolding T twl_struct_invs_init_def by auto
-  then have [simp]: 
+  then have [simp]:
    \<open>cdcl\<^sub>W_restart_mset.cdcl\<^sub>W_all_struct_inv (M, add_mset (mset C) (clauses N + NE + OC),
      clauses U + UE, None)\<close> and
    n_d: \<open>no_dup M\<close>
@@ -1027,12 +1079,14 @@ proof -
 qed
 
 lemma init_dt_pre_add_to_clauses_init_l:
-  assumes 
+  assumes
     D: \<open>get_conflict_l_init S = None\<close> and
     a: \<open>length a \<noteq> Suc 0\<close> \<open>a \<noteq> []\<close> and
     pre: \<open>init_dt_pre (a # CS) S\<close> and
     \<open>\<forall>s\<in>set (get_trail_l_init S). \<not> is_decided s\<close>
-  shows \<open>add_to_clauses_init_l a S \<le> SPEC (init_dt_pre CS)\<close>
+  shows
+    \<open>add_to_clauses_init_l a S \<le> SPEC (init_dt_pre CS)\<close> (is ?pre) and
+    \<open>add_to_clauses_init_l a S \<le> SPEC (init_dt_spec [a] S)\<close> (is ?spec)
 proof -
   obtain T where
     SOC_T: \<open>(S, T) \<in> twl_st_l_init\<close> and
@@ -1054,8 +1108,11 @@ proof -
     using D WS by (cases S) auto
   have le_2: \<open>length a \<ge> 2\<close>
     using a by (cases a) auto
-  have \<open>init_dt_pre CS ((M, fmupd i (a, True) N, None, NE, UE, {#}, Q), OC)\<close>
-    if 
+  have
+    \<open>init_dt_pre CS ((M, fmupd i (a, True) N, None, NE, UE, {#}, Q), OC)\<close> (is ?pre1) and
+    \<open>init_dt_spec [a] S
+          ((M, fmupd i (a, True) N, None, NE, UE, {#}, Q), OC)\<close> (is ?spec1)
+    if
       i_0: \<open>0 < i\<close> and
       i_dom: \<open>i \<notin># dom_m N\<close>
     for i :: \<open>nat\<close>
@@ -1078,12 +1135,18 @@ proof -
     moreover have \<open>twl_stgy_invs (fst (add_to_clauses_init a T))\<close>
       by (rule twl_stgy_invs_backtrack_lvl_0)
         (use dec SOC_T in \<open>auto simp: S count_decided_0_iff twl_st_l_init twl_st_init\<close>)
-    ultimately show ?thesis
-      unfolding init_dt_pre_def apply -
-      apply (rule exI[of _ \<open>add_to_clauses_init a T\<close>])
-      using dist dec OC'_empty in_literals_to_update by (auto simp: S)
+    ultimately show ?pre1 ?spec1
+      unfolding init_dt_pre_def init_dt_spec_def apply -
+      subgoal
+        apply (rule exI[of _ \<open>add_to_clauses_init a T\<close>])
+        using dist dec OC'_empty in_literals_to_update by (auto simp: S)
+      subgoal
+        apply (rule exI[of _ \<open>add_to_clauses_init a T\<close>])
+        using dist dec OC'_empty in_literals_to_update i_dom i_0 a
+        by (auto simp: S learned_clss_l_mapsto_upd_notin_irrelev ran_m_mapsto_upd_notin)
+      done
   qed
-  then show ?thesis
+  then show ?pre ?spec
     by (auto simp: S add_to_clauses_init_l_def get_fresh_index_def RES_RETURN_RES)
 qed
 
@@ -1116,7 +1179,6 @@ proof -
     using S unfolding SOC by auto
   show ?thesis
   proof (cases \<open>get_conflict_l (fst SOC)\<close>)
-    thm twl_struct_invs_init_propagate_unit_init
     case None
     then show ?thesis
       using pre dec by (auto simp add: Let_def count_decided_0_iff SOC twl_st_l_init twl_st_init
@@ -1124,7 +1186,7 @@ proof -
           init_dt_step_def get_fresh_index_def RES_RETURN_RES
           intro!: init_dt_pre_already_propagated_unit_init_l init_dt_pre_set_conflict_init_l
           init_dt_pre_propagate_unit_init init_dt_pre_add_empty_conflict_init_l
-          init_dt_pre_add_to_clauses_init_l
+          init_dt_pre_add_to_clauses_init_l SPEC_rule_conjI
           dest: init_dt_pre_ConsD in_lits_of_l_defined_litD)
   next
     case  (Some D')
@@ -1141,7 +1203,14 @@ proof -
       using dist inv WS dec  in_literals_to_update add_inv stgy_inv SOC_T
       by (auto simp: S'  count_decided_0_iff
           intro!: twl_struct_invs_init_add_to_other_init)
-    then show ?thesis
+    moreover have \<open>init_dt_spec [a] ((M, N, Some D', NE, UE, {#}, Q), OC)
+        ((M, N, Some D', NE, UE, {#}, Q), add_mset (mset a) OC)\<close>
+      unfolding init_dt_spec_def
+      apply (rule exI[of _ \<open>add_to_other_init a T\<close>])
+      using dist inv WS dec  in_literals_to_update add_inv stgy_inv SOC_T
+      by (auto simp: S'  count_decided_0_iff
+          intro!: twl_struct_invs_init_add_to_other_init)
+    ultimately show ?thesis
       by (auto simp: S init_dt_step_def)
   qed
 qed
@@ -1150,6 +1219,78 @@ lemma [twl_st_l_init]:
   \<open>get_trail_l_init (S, OC) = get_trail_l S\<close>
   \<open>literals_to_update_l_init (S, OC) = literals_to_update_l S\<close>
   by (cases S; auto; fail)+
+
+lemma init_dt_spec_append:
+  assumes
+    spec1: \<open>init_dt_spec CS S T\<close>  and
+    spec: \<open>init_dt_spec CS' T U\<close>
+  shows \<open>init_dt_spec (CS @ CS') S U\<close>
+proof -
+  obtain T' where
+    TT': \<open>(T, T') \<in> twl_st_l_init\<close> and
+    \<open>twl_struct_invs_init T'\<close> and
+    \<open>clauses_to_update_l_init T = {#}\<close> and
+    \<open>\<forall>s\<in>set (get_trail_l_init T). \<not> is_decided s\<close> and
+    \<open>get_conflict_l_init T = None \<longrightarrow>
+     literals_to_update_l_init T = uminus `# lit_of `# mset (get_trail_l_init T)\<close> and
+    clss: \<open>mset `# mset CS + mset `# ran_mf (get_clauses_l_init S) + other_clauses_l_init S +
+     get_unit_clauses_l_init S =
+     mset `# ran_mf (get_clauses_l_init T) + other_clauses_l_init T + get_unit_clauses_l_init T\<close> and
+    learned: \<open>learned_clss_lf (get_clauses_l_init S) = learned_clss_lf (get_clauses_l_init T)\<close> and
+    unit_le: \<open>get_learned_unit_clauses_l_init T = get_learned_unit_clauses_l_init S\<close> and
+    \<open>twl_list_invs (fst T)\<close> and
+    \<open>twl_stgy_invs (fst T')\<close> and
+    \<open>other_clauses_l_init T \<noteq> {#} \<longrightarrow> get_conflict_l_init T \<noteq> None\<close> and
+    empty: \<open>{#} \<in># mset `# mset CS \<longrightarrow> get_conflict_l_init T \<noteq> None\<close> and
+    confl_kept: \<open>get_conflict_l_init S \<noteq> None \<longrightarrow> get_conflict_l_init S = get_conflict_l_init T\<close>
+    using spec1
+    unfolding init_dt_spec_def apply -
+    apply normalize_goal+
+    by metis
+
+  obtain U' where
+    UU': \<open>(U, U') \<in> twl_st_l_init\<close> and
+    struct_invs: \<open>twl_struct_invs_init U'\<close> and
+    WS: \<open>clauses_to_update_l_init U = {#}\<close> and
+    dec: \<open>\<forall>s\<in>set (get_trail_l_init U). \<not> is_decided s\<close> and
+    confl: \<open>get_conflict_l_init U = None \<longrightarrow>
+     literals_to_update_l_init U = uminus `# lit_of `# mset (get_trail_l_init U)\<close> and
+    clss': \<open>mset `# mset CS' + mset `# ran_mf (get_clauses_l_init T) + other_clauses_l_init T +
+     get_unit_clauses_l_init T =
+     mset `# ran_mf (get_clauses_l_init U) + other_clauses_l_init U + get_unit_clauses_l_init U\<close> and
+    learned': \<open>learned_clss_lf (get_clauses_l_init T) = learned_clss_lf (get_clauses_l_init U)\<close> and
+    unit_le': \<open>get_learned_unit_clauses_l_init U = get_learned_unit_clauses_l_init T\<close> and
+    list_invs: \<open>twl_list_invs (fst U)\<close> and
+    stgy_invs: \<open>twl_stgy_invs (fst U')\<close> and
+    oth: \<open>other_clauses_l_init U \<noteq> {#} \<longrightarrow> get_conflict_l_init U \<noteq> None\<close> and
+    empty': \<open>{#} \<in># mset `# mset CS' \<longrightarrow> get_conflict_l_init U \<noteq> None\<close> and
+    confl_kept': \<open>get_conflict_l_init T \<noteq> None \<longrightarrow> get_conflict_l_init T = get_conflict_l_init U\<close>
+    using spec
+    unfolding init_dt_spec_def apply -
+    apply normalize_goal+
+    by metis
+
+  show ?thesis
+    unfolding init_dt_spec_def apply -
+    apply (rule exI[of _ U'])
+    apply (intro conjI)
+    subgoal using UU' .
+    subgoal using struct_invs .
+    subgoal using WS .
+    subgoal using dec .
+    subgoal using confl .
+    subgoal using clss clss'
+      by (smt ab_semigroup_add_class.add.commute ab_semigroup_add_class.add.left_commute
+          image_mset_union mset_append)
+    subgoal using learned' learned by simp
+    subgoal using unit_le unit_le' by simp
+    subgoal using list_invs .
+    subgoal using stgy_invs .
+    subgoal using oth .
+    subgoal using empty empty' oth confl_kept' by auto
+    subgoal using confl_kept confl_kept' by auto
+    done
+qed
 
 lemma init_dt_full:
   fixes CS :: \<open>'v literal list list\<close> and SOC :: \<open>'v twl_st_l_init\<close> and S'
@@ -1163,18 +1304,6 @@ lemma init_dt_full:
     \<open>init_dt_pre CS SOC\<close>
   shows
     \<open>init_dt CS SOC \<le> SPEC (init_dt_spec CS SOC)\<close>
-(*     \<open>twl_struct_invs_init (twl_st_of_init SOC')\<close> and
-    \<open>clauses_to_update_l S' = {#}\<close> and
-    \<open>\<forall>s\<in>set (get_trail_l S'). \<not>is_decided s\<close> and
-    \<open>get_conflict_l S' = None \<longrightarrow> literals_to_update_l S' = uminus `# lit_of `# mset (get_trail_l S')\<close> and
-    \<open>mset `# mset CS + cdcl\<^sub>W_restart_mset.clauses (state\<^sub>W_of (twl_st_of None S)) + OC =
-      cdcl\<^sub>W_restart_mset.clauses (state\<^sub>W_of (twl_st_of None S')) + OC'\<close> and
-    \<open>learned_clss (state\<^sub>W_of (twl_st_of None S')) = learned_clss (state\<^sub>W_of (twl_st_of None S))\<close> and
-    \<open>twl_list_invs S'\<close> and
-    \<open>get_learned_l S' = length (get_clauses_l S') - 1\<close> and
-    \<open>twl_stgy_invs (twl_st_of None S')\<close> and
-    \<open>OC' \<noteq> {#} \<longrightarrow> get_conflict_l S' \<noteq> None\<close> and
-    \<open>{#} \<in># mset `# mset CS \<longrightarrow> get_conflict_l S' \<noteq> None\<close> *)
   using assms unfolding S_def OC_def
 proof (induction CS arbitrary: SOC)
   case Nil
@@ -1183,15 +1312,15 @@ proof (induction CS arbitrary: SOC)
   from Nil
   obtain T where
     T: \<open>(SOC, T) \<in> twl_st_l_init\<close>
-      \<open>Ball (set []) distinct\<close> 
-      \<open>twl_struct_invs_init T\<close> 
-      \<open>clauses_to_update_l_init SOC = {#}\<close> 
-      \<open>\<forall>s\<in>set (get_trail_l_init SOC). \<not> is_decided s\<close> 
+      \<open>Ball (set []) distinct\<close>
+      \<open>twl_struct_invs_init T\<close>
+      \<open>clauses_to_update_l_init SOC = {#}\<close>
+      \<open>\<forall>s\<in>set (get_trail_l_init SOC). \<not> is_decided s\<close>
       \<open>get_conflict_l_init SOC = None \<longrightarrow>
        literals_to_update_l_init SOC =
-       uminus `# lit_of `# mset (get_trail_l_init SOC)\<close> 
-      \<open>twl_list_invs (fst SOC)\<close> 
-      \<open>twl_stgy_invs (fst T)\<close> 
+       uminus `# lit_of `# mset (get_trail_l_init SOC)\<close>
+      \<open>twl_list_invs (fst SOC)\<close>
+      \<open>twl_stgy_invs (fst T)\<close>
       \<open>other_clauses_l_init SOC \<noteq> {#} \<longrightarrow> get_conflict_l_init SOC \<noteq> None\<close>
     unfolding init_dt_pre_def apply -
     apply normalize_goal+
@@ -1208,45 +1337,10 @@ next
   note init_dt_step_def[simp]
   have 1: \<open>init_dt_step a SOC \<le> SPEC (\<lambda>SOC'. init_dt_pre CS SOC' \<and> init_dt_spec [a] SOC SOC')\<close>
     by (rule init_dt_pre_init_dt_step[OF pre])
-  have \<open>init_dt_spec (a # CS) SOC UOC\<close>
-    if pre: \<open>init_dt_pre CS T\<close> and spec: \<open>init_dt_spec CS T UOC\<close> and
-        \<open>init_dt_spec [a] SOC T\<close> for T UOC
-  proof -
-    obtain U OC where UOC: \<open>UOC = (U, OC)\<close> by (cases UOC)
-    obtain S' where
-      UOC_S': \<open>((U, OC), S') \<in> twl_st_l_init\<close> and
-      struct_invs: \<open>twl_struct_invs_init S'\<close> and
-      WS: \<open>clauses_to_update_l U = {#}\<close> and
-      dec: \<open>\<forall>s\<in>set (get_trail_l U). \<not> is_decided s\<close> and
-      confl: \<open>get_conflict_l U = None \<longrightarrow> literals_to_update_l U = uminus `# lit_of `# mset (get_trail_l U)\<close> and
-      CS: \<open>mset `# mset CS + mset `# ran_mf (get_clauses_l (fst T)) + snd T = mset `# ran_mf (get_clauses_l U) + OC\<close> and
-      learned: \<open>learned_clss_lf (get_clauses_l (fst T)) = learned_clss_lf (get_clauses_l U)\<close> and
-      add_invs: \<open>twl_list_invs U\<close> and
-      stgy_invs: \<open>twl_stgy_invs (fst S')\<close> and
-      OC: \<open>OC \<noteq> {#} \<longrightarrow> get_conflict_l U \<noteq> None\<close> and
-      empty_conflict: \<open>{#} \<in># mset `# mset CS \<longrightarrow> get_conflict_l U \<noteq> None\<close>
-      using spec
-      unfolding init_dt_spec_def UOC prod.simps apply -
-      apply normalize_goal+ by presburger
-    show ?thesis
-      unfolding init_dt_spec_def UOC prod.simps apply -
-      apply (rule exI[of _ S'])
-      apply (intro conjI)
-      subgoal using UOC_S' .
-      subgoal using struct_invs .
-      subgoal using WS .
-      subgoal using dec .
-      subgoal using confl .
-      subgoal using CS UOC_S' apply (auto simp: twl_st_l_init twl_st_init) sorry
-      subgoal using learned sorry
-      subgoal using add_invs .
-      subgoal using stgy_invs .
-      subgoal using OC .
-      subgoal using pre empty_conflict apply auto sorry
-      subgoal for S'
-      explore_have
-      sorry
-  qed
+  have 2: \<open>init_dt_spec (a # CS) SOC UOC\<close>
+    if spec: \<open>init_dt_spec CS T UOC\<close> and
+       spec': \<open>init_dt_spec [a] SOC T\<close> for T UOC
+    using init_dt_spec_append[OF spec' spec] by simp
   show ?case
     unfolding init_dt.simps
     apply (rule specify_left)
@@ -1255,524 +1349,10 @@ next
      apply (rule IH)
      apply (solves \<open>simp\<close>)
     apply (rule SPEC_rule)
-    thm IH
-
-
-    oops
-
-
-  case 1 then show ?case by simp
-  case 2 then show ?case by simp
-  case 3 then show ?case by simp
-  case 4 then show ?case by simp
-  case 5 then show ?case by (auto simp add: clauses_def)
-  case 6 then show ?case by auto
-  case 7 then show ?case by auto
-  case 8 then show ?case by auto
-  case 9 then show ?case by simp
-  case 10 then show ?case by simp
-  case 11 then show ?case by simp
-next
-  case (Cons a CS) note IH = this(1-)
-  note init_dt_step_def[simp]
-  case 2 note dist = this(1) and inv = this(2) and
-    WS = this(3) and dec = this(4) and in_literals_to_update = this(5) and add_inv = this(6) and
-    len = this(7) and stgy_inv = this(8) and OC'_empty = this(9)
-  let ?SOC' = \<open>init_dt CS (S, OC)\<close>
-  let ?S' = \<open>fst (init_dt CS (S, OC))\<close>
-  let ?OC' = \<open>snd (init_dt CS (S, OC))\<close>
-  have
-    twl: \<open>twl_struct_invs_init (twl_st_of_init ?SOC')\<close> and
-    w_q: \<open>clauses_to_update_l ?S' = {#}\<close> and
-    dec': \<open>\<forall>s\<in>set (get_trail_l ?S'). \<not> is_decided s\<close> and
-    literals_to_update': \<open>get_conflict_l ?S' = None \<longrightarrow>
-        literals_to_update_l ?S' = uminus `# lit_of `# mset (get_trail_l ?S')\<close>
-      and
-    clss': \<open>mset `# mset CS + cdcl\<^sub>W_restart_mset.clauses (state\<^sub>W_of (twl_st_of None S)) + OC =
-      cdcl\<^sub>W_restart_mset.clauses (state\<^sub>W_of (twl_st_of None ?S')) + ?OC'\<close>
-      and
-    learned': \<open>learned_clss (state\<^sub>W_of (twl_st_of None ?S')) = learned_clss (state\<^sub>W_of (twl_st_of None S))\<close>
-      and
-    add_inv': \<open>twl_list_invs ?S'\<close> and
-    U': \<open>get_learned_l ?S' = length (get_clauses_l ?S') - 1\<close> and
-    OC'_empty: \<open>snd ?SOC' \<noteq> {#} \<longrightarrow> get_conflict_l ?S' \<noteq> None\<close>and
-    OC'_empty_conflict: \<open>{#} \<in># mset `# mset CS \<longrightarrow> get_conflict_l ?S' \<noteq> None\<close>
-    using IH[OF _ inv WS dec in_literals_to_update add_inv len stgy_inv OC'_empty] dist by auto
-
-  obtain M N U D NE UE Q OCS where
-    S: \<open>init_dt CS (S, OC) = ((M, N, U, D, NE, UE, {#}, Q), OCS)\<close>
-    using w_q by (cases \<open>init_dt CS (S, OC)\<close>) auto
-  obtain M' N' U' D' NE' WS' UE' Q' where
-    S': \<open>twl_st_of None (fst (init_dt (a # CS) (S, OC))) = (M', N', U', D', NE', UE', WS', Q')\<close>
-    by (cases \<open>twl_st_of None (fst (init_dt (a # CS) (S, OC)))\<close>) auto
-  then have [simp]: \<open>UE' = UE\<close>
-    by (cases a; cases D) (auto simp: S split: if_splits)
-
-  have dec_M: \<open>\<forall>s\<in>set M. \<not> is_decided s\<close>
-    using dec' S by auto
-  have N_not_empty: \<open>N \<noteq> []\<close>
-    using add_inv' unfolding twl_list_invs_def S by auto
-  have U_len_N: \<open>U = length N - 1\<close>
-    using U' unfolding S by auto
-  then have [simp]: \<open>take U (tl N) = tl N\<close> \<open>drop (Suc U) N = []\<close> \<open>drop U (tl N) = []\<close>
-    by auto
-  show ?case using w_q
-    by (cases D) (auto simp: S Let_def)
-  case 3
-  show ?case
-    using dec_M by (cases D) (auto simp: S Let_def)
-  case 4
-  show ?case
-    using literals_to_update' by (cases D) (auto simp: S Let_def)
-  have a_D: \<open>\<exists>x y a'. a = x # y # a'\<close> if \<open>\<forall>L. a \<noteq> [L]\<close> and \<open>a \<noteq> []\<close>
-    apply (case_tac a, (use that in simp; fail))
-    apply (rename_tac aa list, case_tac list; use that in simp)
-    done
-  have mset_tl_N: \<open>{#mset (watched_l x) + mset (unwatched_l x). x \<in># mset (take U (tl N))#} + {#mset (watched_l x) + mset (unwatched_l x). x \<in># mset (drop (Suc U) N)#} =
-         {#mset (watched_l x) + mset (unwatched_l x). x \<in># mset (tl N)#}\<close>
-    unfolding image_mset_union[symmetric] mset_append[symmetric] append_take_drop_id drop_Suc ..
-  case 5
-  show ?case
-    using clss' U_len_N N_not_empty by (cases D)
-      (auto simp: S Let_def clauses_def length_list_Suc_0 cdcl\<^sub>W_restart_mset_state mset_tl_N
-        dest!: a_D)
-  case 6
-  show ?case
-    using learned' U_len_N by (cases D) (auto simp: S Let_def clauses_def length_list_Suc_0
-        cdcl\<^sub>W_restart_mset_state)
-
-  case 7
-  show ?case
-    using add_inv' N_not_empty
-    by (cases D) (fastforce simp add: U_len_N S clauses_def twl_list_invs_def Let_def nth_append
-        cdcl\<^sub>W_restart_mset_state)+
-  case 8
-  show ?case
-    by (cases D) (auto simp add: U_len_N S clauses_def twl_list_invs_def Let_def nth_append
-        cdcl\<^sub>W_restart_mset_state)
-
-  let ?S' = \<open>(convert_lits_l N M, twl_clause_of `# mset (take U (tl N)),
-       twl_clause_of `# mset (drop U (tl N)), D, NE, UE, {#}, Q)\<close>
-  case 1
-  let ?S' = \<open>((convert_lits_l N M, twl_clause_of `# mset (take U (tl N)), twl_clause_of `# mset (drop U (tl N)), D, NE, UE, {#}, Q), OCS)\<close>
-  let ?T' = \<open>state\<^sub>W_of_init ?S'\<close>
-  have
-    struct: \<open>Multiset.Ball (twl_clause_of `# mset (tl N)) struct_wf_twl_cls\<close> and
-    H: \<open>\<forall>C\<in>#twl_clause_of `# mset (tl N). D = None \<longrightarrow>
-      \<not> twl_is_an_exception C Q ({#} :: ('v literal \<times> 'v twl_cls) multiset ) \<longrightarrow>
-      (twl_lazy_update (convert_lits_l N M) C \<and> twl_inv (convert_lits_l N M) C)\<close> and
-    lev: \<open>\<forall>C\<in>#twl_clause_of `# mset (tl N). D = None \<longrightarrow> watched_literals_false_of_max_level (convert_lits_l N M) C\<close> and
-    valid: \<open>valid_enqueued (fst ?S')\<close> and
-    all_struct: \<open>cdcl\<^sub>W_restart_mset.cdcl\<^sub>W_all_struct_inv ?T'\<close> and
-    no_smaller: \<open>cdcl\<^sub>W_restart_mset.no_smaller_propa ?T'\<close> and
-    excep: \<open>twl_st_exception_inv (fst ?S')\<close> and
-    no_dup: \<open>no_duplicate_queued (fst ?S')\<close> and
-    dist_q: \<open>distinct_queued (fst ?S')\<close> and
-    confl_cands: \<open>confl_cands_enqueued (fst ?S')\<close> and
-    propa_cands: \<open>propa_cands_enqueued (fst ?S')\<close> and
-    get_confl: \<open>get_conflict (fst ?S') \<noteq> None \<longrightarrow> clauses_to_update (fst ?S') = {#} \<and>
-    literals_to_update (fst ?S') = {#}\<close> and
-    unit_clss: \<open>entailed_clss_inv (fst ?S')\<close> and
-    w_q: \<open>clauses_to_update_inv (fst ?S')\<close> and
-    past_invs: \<open>past_invs (fst ?S')\<close>
-    using twl unfolding twl_st_inv.simps twl_struct_invs_init_def S twl_st_of.simps
-    image_mset_union[symmetric] mset_append[symmetric] append_take_drop_id drop_Suc S
-    twl_struct_invs_def fst_conv twl_st_of_init.simps by fast+
-
-  have [simp]: \<open>get_level M L = 0\<close> and
-    [simp]: \<open>count_decided M = 0\<close> for L
-    using dec' S by (auto simp: count_decided_0_iff)
-  have nm: \<open>\<forall>s\<in>set (convert_lits_l N M). \<not> is_decided s\<close>
-      using dec_M by (auto simp: convert_lits_l_def)
-  have convert_append_Decided_cons[iff]:
-    \<open>convert_lits_l N M = M'a @ Decided K # Ma \<longleftrightarrow> False\<close>
-    \<open>Propagated L C # convert_lits_l N M = M'a @ Decided K # Ma \<longleftrightarrow> False\<close>
-    for M'a K Ma L C
-    using nm apply fastforce
-    by (metis (no_types, lifting) nm annotated_lit.disc(1)
-          annotated_lit.distinct(1) append_eq_Cons_conv in_set_conv_decomp list_tail_coinc)
-  have
-    alien: \<open>cdcl\<^sub>W_restart_mset.no_strange_atm ?T'\<close> and
-    lev_inv: \<open>cdcl\<^sub>W_restart_mset.cdcl\<^sub>W_M_level_inv ?T'\<close> and
-    learned_tauto: \<open>(\<forall>s\<in>#learned_clss ?T'. \<not> tautology s)\<close> and
-    \<open>cdcl\<^sub>W_restart_mset.distinct_cdcl\<^sub>W_state ?T'\<close> and
-    confl: \<open>cdcl\<^sub>W_restart_mset.cdcl\<^sub>W_conflicting ?T'\<close> and
-    all_decomp: \<open>all_decomposition_implies_m (cdcl\<^sub>W_restart_mset.clauses ?T')
-     (get_all_ann_decomposition (trail ?T'))\<close> and
-    learned: \<open>cdcl\<^sub>W_restart_mset.cdcl\<^sub>W_learned_clause ?T'\<close>
-    using all_struct unfolding cdcl\<^sub>W_restart_mset.cdcl\<^sub>W_all_struct_inv_def S'[symmetric]
-    by fast+
-  have propagated_trail_decomp_iff[iff]: \<open>a @ Propagated La C # b = Propagated L D # M' \<longleftrightarrow>
-        (a = [] \<and> Propagated La C = Propagated L D \<and> b = M') \<or>
-        (a \<noteq> [] \<and> tl a @ Propagated La C # b = M' \<and> hd a = Propagated L D)\<close> for a b La L C D M'
-    by (cases a) auto
-
-  have ex_two_watched_N: \<open>\<exists>L L'. watched_l x = [L, L']\<close> if \<open>x \<in> set (tl N)\<close> for x
-  proof -
-    have \<open>struct_wf_twl_cls (twl_clause_of x)\<close>
-      using struct that by auto
-    then show ?thesis
-      by (cases \<open>twl_clause_of x\<close>) (auto simp: length_list_2 take_2_if)
-  qed
-
-  have in_M_IN_QD: \<open>- La \<in> lits_of_l M \<Longrightarrow> La \<in># Q\<close> if \<open>D = None\<close> for La
-    using S literals_to_update' that by (auto simp: lits_of_def uminus_lit_swap)
-
-  have \<open>x \<in> set M \<Longrightarrow> convert_lit (N @ N') x = convert_lit N x\<close> for x N'
-    using add_inv' by (cases x) (auto simp: nth_append twl_list_invs_def S)
-  then have [simp]: \<open>convert_lits_l (N @ N') M = convert_lits_l N M\<close> for N'
-    unfolding convert_lits_l_def by auto
-  consider
-    (confl) \<open>D \<noteq> None\<close> |
-    (empty) \<open>D = None\<close> and \<open>a = []\<close> |
-    (True) \<open>D = None\<close> and \<open>length a = 1\<close> |
-    (False) \<open>D = None\<close> and \<open>length a \<ge> 2\<close>
-    by (cases a; cases \<open>tl a\<close>) auto
-  then show ?case
-  proof cases
-    case confl
-    then show ?thesis
-      using S' twl dist by (auto simp: S cdcl\<^sub>W_restart_mset_state
-          intro!: twl_struct_invs_init_add_mset)
-  next
-    case a: empty
-    have [simp]: \<open>NE' = NE\<close>
-    using S' by (cases D) (auto simp: a S split: if_splits)
-  note in_M_IN_QD = in_M_IN_QD[OF a(1)]
-  have all_inv':
-    \<open>cdcl\<^sub>W_restart_mset.cdcl\<^sub>W_all_struct_inv (convert_lits_l N M,
-      add_mset {#}
-       ({#mset (watched_l x) + mset (unwatched_l x). x \<in># mset (tl N)#} + NE' + OCS),
-      UE', Some {#})\<close>
-    unfolding cdcl\<^sub>W_restart_mset.cdcl\<^sub>W_all_struct_inv_def S'[symmetric]
-    apply (intro conjI)
-    subgoal
-      using alien by (auto simp: a S cdcl\<^sub>W_restart_mset.no_strange_atm_def cdcl\<^sub>W_restart_mset_state
-          cdcl\<^sub>W_restart_mset.cdcl\<^sub>W_all_struct_inv_def Let_def
-          mset_take_mset_drop_mset atms_of_def
-          dest: in_lits_of_l_defined_litD split: if_splits)
-    subgoal
-      using all_struct by (auto simp: cdcl\<^sub>W_restart_mset.cdcl\<^sub>W_M_level_inv_def cdcl\<^sub>W_restart_mset_state
-          cdcl\<^sub>W_restart_mset.cdcl\<^sub>W_all_struct_inv_def S Let_def split: if_splits)
-    subgoal
-      using all_struct by (auto simp: cdcl\<^sub>W_restart_mset.no_strange_atm_def cdcl\<^sub>W_restart_mset_state
-          cdcl\<^sub>W_restart_mset.cdcl\<^sub>W_all_struct_inv_def S Let_def split: if_splits)
-    subgoal
-      using all_struct by (auto simp: cdcl\<^sub>W_restart_mset_state
-          cdcl\<^sub>W_restart_mset.cdcl\<^sub>W_all_struct_inv_def a S Let_def cdcl\<^sub>W_restart_mset.distinct_cdcl\<^sub>W_state_def
-          split: if_splits)
-    subgoal
-      using confl by (auto simp: a cdcl\<^sub>W_restart_mset.cdcl\<^sub>W_conflicting_def cdcl\<^sub>W_restart_mset_state
-          cdcl\<^sub>W_restart_mset.cdcl\<^sub>W_all_struct_inv_def S Let_def Decided_Propagated_in_iff_in_lits_of_l
-          split: if_splits)
-    subgoal
-      apply (cases \<open>get_all_ann_decomposition (convert_lits_l N M)\<close>)
-      using all_decomp by (auto simp: a cdcl\<^sub>W_restart_mset.no_strange_atm_def cdcl\<^sub>W_restart_mset_state
-          cdcl\<^sub>W_restart_mset.cdcl\<^sub>W_all_struct_inv_def S Let_def clauses_def
-          intro!: all_decomposition_implies_insert_single
-          split: if_splits)
-    subgoal
-      using learned by (auto 5 5 simp: a cdcl\<^sub>W_restart_mset.no_strange_atm_def cdcl\<^sub>W_restart_mset_state
-          cdcl\<^sub>W_restart_mset.cdcl\<^sub>W_all_struct_inv_def S Let_def image_Un
-          cdcl\<^sub>W_restart_mset.cdcl\<^sub>W_learned_clause_def clauses_def
-          split: if_splits)
-    done
-  show ?thesis
-    unfolding twl_struct_invs_init_def S' twl_st_inv.simps
-    apply (intro conjI)
-    subgoal
-      using H S' dec' nm struct by (auto simp: twl_struct_invs_def a S twl_st_inv.simps
-          split: if_splits)
-    subgoal
-      using struct S' by (auto simp: a S split: if_splits)[]
-    subgoal using all_inv' by (auto simp: twl_struct_invs_def a S twl_st_inv.simps
-          split: if_splits)
-    subgoal
-      using S' no_smaller by (auto simp: a S cdcl\<^sub>W_restart_mset_state
-          cdcl\<^sub>W_restart_mset.no_smaller_propa_def clauses_def split: if_splits)
-    subgoal
-      using S' excep by (force simp: a S twl_exception_inv.simps split: if_splits)
-    subgoal
-      using S' by (auto simp: a S split: if_splits)
-    subgoal
-      using S' excep by (force simp: a S twl_exception_inv.simps split: if_splits)
-    subgoal
-      using S' no_dup by (auto simp: a S cdcl\<^sub>W_restart_mset_state
-          twl_exception_inv.simps uminus_lit_swap
-          cdcl\<^sub>W_restart_mset.no_smaller_propa_def clauses_def split: if_splits)
-    subgoal
-      using S' dist_q literals_to_update' by (auto simp add: a S cdcl\<^sub>W_restart_mset_state
-          twl_exception_inv.simps Decided_Propagated_in_iff_in_lits_of_l lits_of_def
-          cdcl\<^sub>W_restart_mset.no_smaller_propa_def clauses_def split: if_splits)
-    subgoal
-      using S' confl_cands by (auto simp: a S cdcl\<^sub>W_restart_mset_state
-          twl_exception_inv.simps uminus_lit_swap true_annots_true_cls_def_iff_negation_in_model
-          cdcl\<^sub>W_restart_mset.no_smaller_propa_def clauses_def conj_disj_distribR ex_disj_distrib
-          dest: in_diffD dest!: in_M_IN_QD dest!: ex_two_watched_N
-          split: if_splits)
-    subgoal
-      using S' propa_cands unit_clss by (auto simp: a S cdcl\<^sub>W_restart_mset_state
-          twl_exception_inv.simps uminus_lit_swap true_annots_true_cls_def_iff_negation_in_model
-          cdcl\<^sub>W_restart_mset.no_smaller_propa_def clauses_def conj_disj_distribR ex_disj_distrib
-          dest: in_diffD dest!: in_M_IN_QD dest!: ex_two_watched_N
-          split: if_splits)
-    subgoal
-      using S' by (auto simp: a S cdcl\<^sub>W_restart_mset_state
-          twl_exception_inv.simps uminus_lit_swap
-          cdcl\<^sub>W_restart_mset.no_smaller_propa_def clauses_def split: if_splits)
-    subgoal
-      using S' past_invs by (auto simp: a S past_invs.simps
-          cdcl\<^sub>W_restart_mset.no_smaller_propa_def clauses_def split: if_splits)
-    done
-  next
-    case True note _[simp] = this(1) and a = this(2)
-    then obtain L where a: \<open>a = [L]\<close>
-      using list_decomp_1 by blast
-    note in_M_IN_QD = in_M_IN_QD[OF True(1)]
-    have all_inv':
-      \<open>cdcl\<^sub>W_restart_mset.cdcl\<^sub>W_all_struct_inv (state\<^sub>W_of_init (twl_st_of_init (init_dt (a # CS) (S, OC))))\<close>
-      unfolding cdcl\<^sub>W_restart_mset.cdcl\<^sub>W_all_struct_inv_def S'[symmetric]
-        init_dt.simps S
-      apply (intro conjI)
-      subgoal
-        using alien by (auto simp: a S cdcl\<^sub>W_restart_mset.no_strange_atm_def cdcl\<^sub>W_restart_mset_state
-            cdcl\<^sub>W_restart_mset.cdcl\<^sub>W_all_struct_inv_def Let_def dest: in_lits_of_l_defined_litD split: if_splits)
-      subgoal
-        using all_struct by (auto simp: cdcl\<^sub>W_restart_mset.cdcl\<^sub>W_M_level_inv_def cdcl\<^sub>W_restart_mset_state
-            cdcl\<^sub>W_restart_mset.cdcl\<^sub>W_all_struct_inv_def S Let_def split: if_splits)
-      subgoal
-        using all_struct by (auto simp: cdcl\<^sub>W_restart_mset.no_strange_atm_def cdcl\<^sub>W_restart_mset_state
-            cdcl\<^sub>W_restart_mset.cdcl\<^sub>W_all_struct_inv_def S Let_def split: if_splits)
-      subgoal
-        using all_struct by (auto simp: cdcl\<^sub>W_restart_mset_state
-            cdcl\<^sub>W_restart_mset.cdcl\<^sub>W_all_struct_inv_def a S Let_def cdcl\<^sub>W_restart_mset.distinct_cdcl\<^sub>W_state_def
-            split: if_splits)
-      subgoal
-        using confl by (auto simp: a cdcl\<^sub>W_restart_mset.cdcl\<^sub>W_conflicting_def cdcl\<^sub>W_restart_mset_state
-            cdcl\<^sub>W_restart_mset.cdcl\<^sub>W_all_struct_inv_def S Let_def Decided_Propagated_in_iff_in_lits_of_l
-            split: if_splits)
-      subgoal
-        apply (cases \<open>get_all_ann_decomposition (convert_lits_l N M)\<close>)
-        using all_decomp by (auto simp: a cdcl\<^sub>W_restart_mset.no_strange_atm_def cdcl\<^sub>W_restart_mset_state
-            cdcl\<^sub>W_restart_mset.cdcl\<^sub>W_all_struct_inv_def S Let_def clauses_def
-            intro!: all_decomposition_implies_insert_single
-            split: if_splits)
-      subgoal
-        using learned by (auto simp: a cdcl\<^sub>W_restart_mset.no_strange_atm_def cdcl\<^sub>W_restart_mset_state
-            cdcl\<^sub>W_restart_mset.cdcl\<^sub>W_all_struct_inv_def S Let_def
-            cdcl\<^sub>W_restart_mset.cdcl\<^sub>W_learned_clause_def clauses_def
-            split: if_splits)
-      done
-    show ?thesis
-      unfolding twl_struct_invs_init_def S' twl_st_inv.simps
-      apply (intro conjI)
-      subgoal
-        using H S' dec' nm struct by (auto simp: twl_struct_invs_def a S twl_st_inv.simps
-            split: if_splits)
-      subgoal
-        using H S' valid by (auto simp: twl_struct_invs_def a S twl_st_inv.simps
-            get_level_cons_if split: if_splits)
-      subgoal using all_inv'
-        using S' by (auto simp: a S cdcl\<^sub>W_restart_mset_state
-            twl_exception_inv.simps uminus_lit_swap
-            cdcl\<^sub>W_restart_mset.no_smaller_propa_def clauses_def split: if_splits)
-      subgoal
-        using S' no_smaller by (auto simp: a S cdcl\<^sub>W_restart_mset_state
-            cdcl\<^sub>W_restart_mset.no_smaller_propa_def clauses_def split: if_splits)
-      subgoal
-        using S' excep by (force simp: a S twl_exception_inv.simps split: if_splits)
-      subgoal
-        using S' no_dup by (auto simp: a S cdcl\<^sub>W_restart_mset_state
-            twl_exception_inv.simps uminus_lit_swap
-            cdcl\<^sub>W_restart_mset.no_smaller_propa_def clauses_def split: if_splits)
-      subgoal
-        using S' dist_q literals_to_update' by (auto simp add: a S cdcl\<^sub>W_restart_mset_state
-            twl_exception_inv.simps Decided_Propagated_in_iff_in_lits_of_l lits_of_def
-            cdcl\<^sub>W_restart_mset.no_smaller_propa_def clauses_def split: if_splits)
-      subgoal
-        using S' confl_cands by (auto simp: a S cdcl\<^sub>W_restart_mset_state
-            twl_exception_inv.simps uminus_lit_swap true_annots_true_cls_def_iff_negation_in_model
-            cdcl\<^sub>W_restart_mset.no_smaller_propa_def clauses_def conj_disj_distribR ex_disj_distrib
-            dest: in_diffD dest!: in_M_IN_QD dest!: ex_two_watched_N
-            split: if_splits)
-      subgoal
-        using S' propa_cands by (auto simp: a S cdcl\<^sub>W_restart_mset_state
-            twl_exception_inv.simps uminus_lit_swap true_annots_true_cls_def_iff_negation_in_model
-            cdcl\<^sub>W_restart_mset.no_smaller_propa_def clauses_def conj_disj_distribR ex_disj_distrib
-            dest: in_diffD dest!: in_M_IN_QD dest!: ex_two_watched_N
-            split: if_splits)
-      subgoal
-        using struct S' by (auto simp: a S split: if_splits)[]
-      subgoal
-        using S' unit_clss by (auto 3 3 simp: a S cdcl\<^sub>W_restart_mset_state
-            twl_exception_inv.simps uminus_lit_swap get_level_cons_if
-            cdcl\<^sub>W_restart_mset.no_smaller_propa_def clauses_def split: if_splits)
-      subgoal
-        using S' w_q by (auto simp: a S cdcl\<^sub>W_restart_mset_state
-            twl_exception_inv.simps uminus_lit_swap get_level_cons_if filter_mset_empty_conv
-            clauses_to_update_prop.simps
-            cdcl\<^sub>W_restart_mset.no_smaller_propa_def clauses_def split: if_splits
-            dest: in_M_IN_QD)
-      subgoal
-        using S' past_invs by (auto simp: a S past_invs.simps
-            cdcl\<^sub>W_restart_mset.no_smaller_propa_def clauses_def split: if_splits)
-      done
-  next
-    case False note [simp] = this(1) and a = this(2)
-    then have [simp]: \<open>length a \<noteq> Suc 0\<close> by auto
-    then obtain x y a' where a: \<open>a = x # y # a'\<close>
-      apply (case_tac a, (use False in simp; fail))
-      apply (rename_tac aa list, case_tac list; simp)
-      done
-    have all_inv':
-      \<open>cdcl\<^sub>W_restart_mset.cdcl\<^sub>W_all_struct_inv (state\<^sub>W_of_init (twl_st_of_init (init_dt (a # CS) (S, OC))))\<close>
-      unfolding cdcl\<^sub>W_restart_mset.cdcl\<^sub>W_all_struct_inv_def S'[symmetric]
-      apply (intro conjI)
-      subgoal
-        using alien N_not_empty
-        by (auto 3 3 simp: a S cdcl\<^sub>W_restart_mset.no_strange_atm_def cdcl\<^sub>W_restart_mset_state
-            cdcl\<^sub>W_restart_mset.cdcl\<^sub>W_all_struct_inv_def Let_def dest: (* in_lits_of_l_defined_litD *)
-            split: if_splits)
-      subgoal
-        using all_struct by (auto simp: cdcl\<^sub>W_restart_mset.cdcl\<^sub>W_M_level_inv_def cdcl\<^sub>W_restart_mset_state
-            cdcl\<^sub>W_restart_mset.cdcl\<^sub>W_all_struct_inv_def S Let_def split: if_splits)
-      subgoal
-        using all_struct by (auto simp: cdcl\<^sub>W_restart_mset.no_strange_atm_def cdcl\<^sub>W_restart_mset_state
-            cdcl\<^sub>W_restart_mset.cdcl\<^sub>W_all_struct_inv_def S Let_def split: if_splits)
-      subgoal
-        using all_struct dist N_not_empty by (auto simp: cdcl\<^sub>W_restart_mset_state
-            cdcl\<^sub>W_restart_mset.cdcl\<^sub>W_all_struct_inv_def a S Let_def cdcl\<^sub>W_restart_mset.distinct_cdcl\<^sub>W_state_def
-            convert_lits_l_append split: if_splits)
-      subgoal
-        using confl by (auto simp: a cdcl\<^sub>W_restart_mset.cdcl\<^sub>W_conflicting_def cdcl\<^sub>W_restart_mset_state
-            cdcl\<^sub>W_restart_mset.cdcl\<^sub>W_all_struct_inv_def S Let_def propagated_trail_decomp_iff
-            Decided_Propagated_in_iff_in_lits_of_l
-            split: if_splits)
-      subgoal
-        apply (cases \<open>get_all_ann_decomposition (convert_lits_l N M)\<close>)
-        using all_decomp N_not_empty by (auto simp: a cdcl\<^sub>W_restart_mset.no_strange_atm_def cdcl\<^sub>W_restart_mset_state
-            cdcl\<^sub>W_restart_mset.cdcl\<^sub>W_all_struct_inv_def S Let_def clauses_def
-            intro!: all_decomposition_implies_insert_single
-            split: if_splits)
-      subgoal
-        using learned N_not_empty by (auto simp: a cdcl\<^sub>W_restart_mset.no_strange_atm_def cdcl\<^sub>W_restart_mset_state
-            cdcl\<^sub>W_restart_mset.cdcl\<^sub>W_all_struct_inv_def S Let_def
-            cdcl\<^sub>W_restart_mset.cdcl\<^sub>W_learned_clause_def clauses_def
-            split: if_splits)
-      done
-    show ?thesis
-      unfolding twl_struct_invs_init_def S' twl_st_inv.simps
-      apply (intro conjI)
-      subgoal
-        using H S' dec struct N_not_empty dist by (auto simp: twl_struct_invs_def a S twl_st_inv.simps
-            split: if_splits)
-      subgoal
-        using H S' valid by (auto simp: twl_struct_invs_def a S twl_st_inv.simps
-            get_level_cons_if
-            split: if_splits)
-      subgoal using all_inv' .
-      subgoal
-        using S' no_smaller by (auto simp: a S cdcl\<^sub>W_restart_mset_state
-            cdcl\<^sub>W_restart_mset.no_smaller_propa_def clauses_def split: if_splits)
-      subgoal
-        using S' excep in_M_IN_QD by (auto simp: a S cdcl\<^sub>W_restart_mset_state
-            twl_exception_inv.simps uminus_lit_swap add_mset_eq_add_mset
-            cdcl\<^sub>W_restart_mset.no_smaller_propa_def clauses_def
-            split: if_splits)
-      subgoal
-        using S' no_dup by (auto simp: a S cdcl\<^sub>W_restart_mset_state
-            twl_exception_inv.simps uminus_lit_swap
-            cdcl\<^sub>W_restart_mset.no_smaller_propa_def clauses_def split: if_splits)
-      subgoal
-        using S' dist_q in_literals_to_update by (auto simp add: a S cdcl\<^sub>W_restart_mset_state
-            twl_exception_inv.simps Decided_Propagated_in_iff_in_lits_of_l lits_of_def
-            cdcl\<^sub>W_restart_mset.no_smaller_propa_def clauses_def split: if_splits)
-      subgoal
-        using S' confl_cands in_M_IN_QD N_not_empty by (force simp: a S cdcl\<^sub>W_restart_mset_state
-            twl_exception_inv.simps uminus_lit_swap ex_disj_distrib conj_disj_distribR
-            cdcl\<^sub>W_restart_mset.no_smaller_propa_def clauses_def
-            dest!: in_M_IN_QD dest!: ex_two_watched_N
-            split: if_splits)+
-      subgoal
-        using S' propa_cands in_M_IN_QD N_not_empty by (auto simp: a S cdcl\<^sub>W_restart_mset_state
-            twl_exception_inv.simps uminus_lit_swap ex_disj_distrib conj_disj_distribR
-            all_conj_distrib cdcl\<^sub>W_restart_mset.no_smaller_propa_def clauses_def
-            dest!: ex_two_watched_N split: if_splits)
-      subgoal by (auto simp: S Let_def a split: if_splits)
-
-      subgoal
-        using S' unit_clss by (cases D) (auto simp: a S cdcl\<^sub>W_restart_mset_state
-            twl_exception_inv.simps uminus_lit_swap get_level_cons_if
-            cdcl\<^sub>W_restart_mset.no_smaller_propa_def clauses_def split: if_splits)
-      subgoal
-        using S' w_q in_M_IN_QD by (cases D) (auto simp: a S cdcl\<^sub>W_restart_mset_state
-            twl_exception_inv.simps uminus_lit_swap get_level_cons_if filter_mset_empty_conv
-            clauses_to_update_prop.simps
-            cdcl\<^sub>W_restart_mset.no_smaller_propa_def clauses_def
-            split: if_splits)
-      subgoal
-        apply (cases D)
-        using S' past_invs by (auto simp: a S past_invs.simps
-            cdcl\<^sub>W_restart_mset.no_smaller_propa_def clauses_def split: if_splits)
-      done
-  qed
-  case 9
-  show ?case
-    unfolding twl_stgy_invs_def cdcl\<^sub>W_restart_mset.cdcl\<^sub>W_stgy_invariant_def
-       cdcl\<^sub>W_restart_mset.conflict_non_zero_unless_level_0_def
-    by (cases D; cases a)
-        (auto simp: S cdcl\<^sub>W_restart_mset.no_smaller_confl_def clauses_def
-        cdcl\<^sub>W_restart_mset_state Let_def)
-
-  case 10
-  show ?case
-    using OC'_empty
-    by (cases D; cases a) (auto simp: S cdcl\<^sub>W_restart_mset_state Let_def)
-  case 11
-  show ?case
-    using OC'_empty_conflict
-    by (cases D; cases a) (auto simp: S cdcl\<^sub>W_restart_mset_state Let_def)
+    by (rule 2) fast+
 qed
 
-lemma clauses_init_dt_not_Nil: \<open>fst (snd (fst (init_dt CS (([], [[]], 0, None, {#}, {#}, {#}, {#}), OC)))) \<noteq> []\<close>
-  apply (induction CS)
-  subgoal by (auto simp: init_dt_step_def)
-  subgoal for C CS
-    by (cases \<open>init_dt CS (([], [[]], 0, None, {#}, {#}, {#}, {#}), OC)\<close>)
-     (auto simp: init_dt_step_def Let_def split: option.splits if_splits)
-  done
-
-lemma init_dt_conflict_remains:
-  fixes CS :: \<open>'v literal list list\<close> and S :: \<open>'v twl_st_l\<close> and OC :: \<open>'v clauses\<close>
-  defines \<open>S' \<equiv> fst (init_dt CS (S, OC))\<close>
-  shows \<open>get_conflict_l S \<noteq> None \<longrightarrow> get_conflict_l S = get_conflict_l S'\<close>
-  unfolding S'_def apply (induction CS)
-  subgoal by simp
-  subgoal for a CS
-    by (cases \<open>init_dt CS (S, OC)\<close>; cases \<open>get_conflict_l S\<close>)
-      (auto simp: init_dt_step_def Let_def split: option.splits if_splits)
-  done
-
-lemma init_dt_confl_in_clauses:
-  fixes CS :: \<open>'v literal list list\<close> and S :: \<open>'v twl_st_l\<close> and OC :: \<open>'v clauses\<close>
-  defines \<open>S' \<equiv> fst (init_dt CS (S, OC))\<close>
-  assumes
-    \<open>get_conflict_l S \<noteq> None \<longrightarrow> the (get_conflict_l S) \<in># mset `# mset CS\<close>
-  shows
-    \<open>get_conflict_l S' \<noteq> None \<longrightarrow> the (get_conflict_l S') \<in># mset `# mset CS\<close>
-  using assms(2-) unfolding S'_def apply (induction CS)
-  subgoal by simp
-  subgoal for a CS
-    using init_dt_conflict_remains[of S CS OC]
-    by (cases \<open>init_dt CS (S, OC)\<close>; cases \<open>get_conflict_l S\<close>)
-      (auto simp: init_dt_step_def Let_def split: option.splits if_splits)
-  done
-
-lemma clauses_state\<^sub>W_of_init_clauses_state\<^sub>W_of:
-  \<open>cdcl\<^sub>W_restart_mset.clauses (state\<^sub>W_of_init (twl_st_of_init S)) =
-    cdcl\<^sub>W_restart_mset.clauses (state\<^sub>W_of (twl_st_of None (fst S))) + snd S\<close>
-  by (cases S)  (auto simp: clauses_def)
-
+(* TODO needs to be done via proper refinement!
 theorem init_dt:
   fixes CS S
   defines S: \<open>S \<equiv> (([], [[]], 0, None, {#}, {#}, {#}, {#}), {#})\<close>
@@ -1846,5 +1426,5 @@ proof -
     by (rule init_dt_full(11)[of CS \<open>fst S\<close> \<open>snd S\<close>, OF assms(2),
       unfolded prod.collapse]) auto
 qed
-
+*)
 end
